\section{List of isomorphisms}\label{list-of-isomorphisms}

\subsection{Linear negation}\label{linear-negation-1}

\(\begin{array}{rclcrcl}
  A\biorth &amp;\cong&amp; A\\
  (A\tens B)\orth &amp;\cong&amp; A\orth\parr B\orth &amp;\quad&amp; \one\orth  &amp;\cong&amp; \bot\\
  (A\parr B)\orth &amp;\cong&amp; A\orth\tens B\orth &amp;\quad&amp; \bot\orth  &amp;\cong&amp; \one\\
  (A\with B)\orth &amp;\cong&amp; A\orth\plus B\orth &amp;\quad&amp; \top\orth  &amp;\cong&amp; \zero\\
  (A\plus B)\orth &amp;\cong&amp; A\orth\with B\orth &amp;\quad&amp; \zero\orth &amp;\cong&amp; \top\\
  (\oc A)\orth &amp;\cong&amp; \wn A\orth\\
  (\wn A)\orth &amp;\cong&amp; \oc A\orth\\
\end{array}\)

\subsection{Neutrals}\label{neutrals}

\(\begin{array}{rcl}
  A\tens\one  &amp;\cong&amp; \one\tens A\cong A\\
  A\parr\bot  &amp;\cong&amp; \bot\parr A\cong A\\
  A\with\top  &amp;\cong&amp; \top\with A\cong A\\
  A\plus\zero &amp;\cong&amp;\zero\plus A\cong A\\
\end{array}\)

\subsection{Commutativity}\label{commutativity-1}

\(\begin{array}{rcl}
  A\tens B &amp;\cong&amp; B\tens A\\
  A\parr B &amp;\cong&amp; B\parr A\\
  A\with B &amp;\cong&amp; B\with A\\
  A\plus B &amp;\cong&amp; B\plus A\\
\end{array}\)

\subsection{Associativity}\label{associativity}

\(\begin{array}{rcl}
  (A\tens B)\tens C &amp;\cong&amp; A\tens(B\tens C)\\
  (A\parr B)\parr C &amp;\cong&amp; A\parr(B\parr C)\\
  (A\with B)\with C &amp;\cong&amp; A\with(B\with C)\\
  (A\plus B)\plus C &amp;\cong&amp; A\plus(B\plus C)\\
\end{array}\)

\subsection{Multiplicative-additive
distributivity}\label{multiplicative-additive-distributivity}

\(\begin{array}{rclcrcl}
  A\tens(B\plus C) &amp;\cong&amp; (A\tens B)\plus(A\tens C) &amp;\quad&amp;
  A\tens\zero &amp;\cong&amp; \zero\\
  A\parr(B\with C) &amp;\cong&amp; (A\parr B)\with(A\parr C) &amp;\quad&amp;
  A\parr\top &amp;\cong&amp; \top\\
\end{array}\)

\subsection{Linear implication}\label{linear-implication}

\(\begin{array}{rclcrcl}
  A\limp B &amp;\cong&amp; A\orth\parr B\\
  A\limp B &amp;\cong&amp; B\orth\limp A\orth\\
  A\tens B \limp C &amp;\cong&amp; A\limp B \limp C\\
\end{array}\)

\subsection{The exponential
isomorphisms}\label{the-exponential-isomorphisms}

\(\begin{array}{rclcrcl}
  \oc(A\with B) &amp;\cong&amp; \oc A\tens\oc B &amp;\quad&amp; \oc\top &amp;\cong&amp; \one\\
  \wn(A\plus B) &amp;\cong&amp; \wn A\parr\wn B &amp;\quad&amp; \wn\zero &amp;\cong&amp; \bot\\
\end{array}\)

\subsection{Quantifiers}\label{quantifiers-1}

\(\begin{array}{rclcrcl}
  \forall \xi_1. \forall\xi_2. A &amp;\cong&amp; \forall\xi_2. \forall\xi_1. A\\
  \exists \xi_1. \exists\xi_2.A &amp;\cong&amp; \exists\xi_2.\exists\xi_1.A\\
\\
  \forall \xi . (A \parr B) &amp;\cong&amp; A \parr \forall \xi.B \quad (\xi\notin A) \\
  \exists \xi . (A \tens B) &amp;\cong&amp; A \tens \exists \xi.B \quad (\xi\notin A) \\
\\
  \forall \xi . (A \with B) &amp;\cong&amp; (\forall \xi . A) \with (\forall \xi . B) &amp; &amp; \forall \xi . \top &amp;\cong&amp; \top \\
  \exists \xi . (A \plus B) &amp;\cong&amp; (\exists \xi . A) \plus (\exists \xi . B) &amp; &amp; \exists \xi . \zero &amp;\cong&amp; \zero
\end{array}\)

